got first pass working

ArrowPoly/ArrowPoly.lean
@@ -9,6 +9,9 @@ structure ATLP where
   normalized : fst ≤ snd
 deriving Repr, Ord
 
+instance : ToString ATLP where
+  toString p := s!"P[{p.fst},{p.snd},{p.whiskers}]"
+
 instance : Inhabited ATLP := ⟨{ fst := 0, snd := 0, whiskers := 0, normalized := Nat.le.refl }⟩
 
 local instance : LT ATLP := ltOfOrd
@@ -25,7 +28,11 @@ def ATLP.toPair (p : ATLP) : Nat × Nat := (p.fst, p.snd)
 def ATLP.indices (p : ATLP) : List Nat := [p.fst, p.snd]
 
 def ATLP.loop_eval (p : ATLP) (h : p.fst = p.snd) : Poly :=
-  (- Poly.A 2 - Poly.A (-2)) * Poly.K p.whiskers.natAbs
+  (- Poly.A 2 - Poly.A (-2)) * Poly.K (p.whiskers.natAbs / 2)
+
+@[simp] theorem ATLP.loop_eval_nonzero (p : ATLP) (h : p.fst = p.snd) :
+  p.loop_eval h ≠ 0 :=
+sorry
 
 def ATLP.combine (p1 p2 : ATLP) : Option ATLP :=
   if p1.fst = p2.fst then
@@ -42,15 +49,47 @@ attribute [local instance] Array.lexicographic
 
 /-- "arrow Templerley-Lieb diagram" -/
 structure ATLD where
+  coeff : Poly
   paths : Array ATLP
+  coeff_nonzero : coeff ≠ 0 := by simp [*]
   ordered : paths |>.map ATLP.toPair |>.strictIncreasing
   nodup : (paths.toList.bind ATLP.indices).nodup
-deriving Repr, Ord
+deriving Repr
 
-instance : Inhabited ATLD :=
-  ⟨{ paths := #[], ordered := Array.strictIncreasing_empty, nodup := List.nodup.nil }⟩
+instance : ToString ATLD where
+  toString d := toString d.coeff ++ " * D[" ++ ",".intercalate (d.paths.map toString).toList ++ "]"
 
-local instance : LT ATLD := ltOfOrd
+def ATLD.one : ATLD where
+  coeff := 1
+  paths := #[]
+  ordered := Array.strictIncreasing_empty
+  nodup := List.nodup.nil
+
+instance : Inhabited ATLD := ⟨ATLD.one⟩
+
+instance : Coe ATLP ATLD where
+  coe p :=
+    if hp : p.fst = p.snd then
+      { coeff := p.loop_eval hp
+        paths := #[],
+        ordered := Array.strictIncreasing_empty,
+        nodup := List.nodup.nil }
+    else
+      { coeff := 1,
+        paths := #[p],
+        ordered := Array.strictIncreasing_singleton _,
+        nodup := by
+          show List.nodup [p.fst, p.snd]
+          apply List.nodup.cons
+          cases p
+          intro h
+          cases h
+          · simp at hp
+          · simp at hp
+            rename_i h'
+            cases h' }
+
+local instance : LT (Array ATLP) := ltOfOrd
 
 def ATLD.concat_path_aux (paths : Array ATLP) (i : Nat) (p : ATLP) (q : Poly) : Poly × Array ATLP :=
   if hi : i < paths.size then
@@ -73,30 +112,157 @@ def ATLD.concat_path_aux (paths : Array ATLP) (i : Nat) (p : ATLP) (q : Poly) : 
     (q, paths.binInsert (· < ·) p)
 termination_by _ => paths.size - i
 
-def ATLD.concat_path (d : ATLD) (p : ATLP) (q : Poly := 1) : Poly × ATLD :=
+def ATLD.concat_path (paths : Array ATLP) (p : ATLP) (q : Poly) : Poly × Array ATLP :=
   if h : p.fst = p.snd then
-    (q * p.loop_eval h, d)
+    (q * p.loop_eval h, paths)
   else
-    let (q', paths') := ATLD.concat_path_aux d.paths 0 p q
-    (q', { paths := paths',
-           ordered := sorry, nodup := sorry })
+    ATLD.concat_path_aux paths 0 p q
 
-def ATLD.concat (d d' : ATLD) (q : Poly := 1) : Poly × ATLD := Id.run do
-  let mut q := q
-  let mut d := d
+def ATLD.concat_aux (d d' : ATLD) : Poly × Array ATLP := Id.run do
+  let mut q := d.coeff * d'.coeff
+  let mut paths := d.paths
   for p in d'.paths do
-    (q, d) := d.concat_path p q
-  return (q, d)
+    (q, paths) := ATLD.concat_path paths p q
+  return (q, paths)
 
+def ATLD.concat (d d' : ATLD) : ATLD :=
+  let (q, paths) := ATLD.concat_aux d d'
+  { coeff := q,
+    paths := paths,
+    coeff_nonzero := sorry,
+    ordered := sorry,
+    nodup := sorry }
 
-/-- Create an ATLD by sorting the input array. -/
-def ATLD.ofArray (paths : Array ATLP) : Poly × ATLD := Id.run do
-  let mut q : Poly := 1
-  let mut d : ATLD := default
+def ATLD.ofArray (paths : Array ATLP) (q : Poly := 1) : ATLD := Id.run do
+  let mut q : Poly := q
+  let mut d : Array ATLP := #[]
   for p in paths do
-    (q, d) := d.concat_path p q
-  return (q, d)
+    (q, d) := ATLD.concat_path d p q
+  return { coeff := q,
+           paths := d,
+           coeff_nonzero := sorry,
+           ordered := sorry,
+           nodup := sorry }
+
+def ATLD.scale (d : ATLD) (q : Poly) (hq : q ≠ 0) : ATLD where
+  coeff := d.coeff * q
+  paths := d.paths
+  coeff_nonzero := sorry
+  ordered := d.ordered
+  nodup := d.nodup
 
 structure ATL where
-  diagrams : Array (ATLD × Poly)
-  ordered : diagrams |>.map Prod.fst |>.strictIncreasing
+  diagrams : Array ATLD
+  ordered : diagrams |>.map ATLD.paths |>.strictIncreasing
+deriving Repr
+
+instance : ToString ATL where
+  toString a := "ATL[" ++ ", ".intercalate (a.diagrams.map toString).toList ++ "]"
+
+def ATL.zero : ATL where
+  diagrams := #[]
+  ordered := Array.strictIncreasing_empty
+
+def ATL.one : ATL where
+  diagrams := #[ATLD.one]
+  ordered := Array.strictIncreasing_singleton _
+
+def ATL.add (x y : ATL) : ATL :=
+  let f (p : Array ATLD) : Merge ATLD → Array ATLD
+    | .left m₁ => p.push m₁
+    | .right m₂ => p.push m₂
+    | .both m₁ m₂ =>
+      let q := m₁.coeff + m₂.coeff
+      if h : q = 0 then
+        p
+      else
+        p.push <| {m₁ with coeff := q, coeff_nonzero := h}
+  let p := Array.mergeBy ATLD.paths f #[] x.diagrams y.diagrams
+  have : (p.map ATLD.paths).strictIncreasing := by
+    sorry
+  ⟨p, this⟩
+
+instance : Add ATL where
+  add := ATL.add
+
+def ATL.scale (x : ATL) (p : Poly) : ATL :=
+  if hp : p = 0 then
+    ATL.zero
+  else
+    { diagrams := x.diagrams.map (λ d => d.scale p hp),
+      ordered := sorry }
+
+def ATL.mulDiagram (x : ATL) (d : ATLD) : ATL := Id.run do
+  let mut diagrams : Array ATLD := #[]
+  for xd in x.diagrams do
+    let d' := xd.concat d
+    diagrams := Id.run <| diagrams.binInsertM' (λ (d1 d2 : ATLD) => d1.paths < d2.paths)
+      (merge := fun d'' =>
+        let c := d'.coeff + d''.coeff
+        if hc : c = 0 then
+          none
+        else
+          some { coeff := c,
+                 paths := d''.paths,
+                 ordered := d''.ordered,
+                 nodup := d''.nodup })
+      (add := fun _ => d')
+      d'
+  return { diagrams := diagrams,
+           ordered := sorry }
+
+def ATL.mul (x y : ATL) : ATL := Id.run do
+  let mut z := ATL.zero
+  for d in y.diagrams do
+    z := z + x.mulDiagram d
+  return z
+
+instance : Mul ATL where
+  mul := ATL.mul
+
+instance : HMul Poly ATL ATL where
+  hMul q t := t.scale q
+
+instance : Coe ATLD ATL where
+  coe d := { diagrams := #[d], ordered := Array.strictIncreasing_singleton _ }
+
+def ATL.P (i j : Nat) (whiskers : Int := 0) : ATL := ATLP.mk' i j whiskers
+
+def ATL.Xp (i j k l : Nat) : ATL :=
+  ATLD.ofArray #[ATLP.mk' i j 0, ATLP.mk' l k 0] (Poly.A 1)
+  + ATLD.ofArray #[ATLP.mk' i l 1, ATLP.mk' j k 1] (Poly.A (-1))
+
+def ATL.Xm (i j k l : Nat) : ATL :=
+  ATLD.ofArray #[ATLP.mk' j k 0, ATLP.mk' i l 0] (Poly.A (-1))
+  + ATLD.ofArray #[ATLP.mk' j i 1, ATLP.mk' k l 1] (Poly.A 1)
+
+def ATL.finalize (a : ATL) : Poly := Id.run do
+  let mut p : Poly := 0
+  for d in a.diagrams do
+    if d.paths.size = 1 then
+      p := p + d.coeff * Poly.K (d.paths[0].whiskers.natAbs / 2)
+    else
+      panic! "ATL.finalize: internal error"
+  return p
+
+def arrow_poly (p : PD Nat) : Poly := Id.run do
+  let mut a : ATL := ATL.one
+  for node in (id p : Array _) do
+    let a' := match node with
+              | .Xp a b c d => ATL.Xp a b c d
+              | .Xm a b c d => ATL.Xm a b c d
+              | .P a b => ATL.P a b
+    a := a * a'
+  return a.finalize
+
+/-
+#eval toString <| (2 : Poly) * ATL.one * ATL.one * (ATLP.mk' 1 2 0 : ATL) * (ATLP.mk' 1 2 0 : ATL)
+
+#eval toString <| ATL.Xp 1 2 3 4
+
+#eval toString <| ATL.finalize <| ATL.Xm 2 0 3 1 * ATL.Xm 3 1 4 2
+
+#eval toString <| ATL.finalize <| ATL.Xm 2 5 1 4 * ATL.Xp 4 0 3 1 * ATL.Xp 6 2 5 3
+
+#eval toString <| ATL.finalize <| ATL.Xp 8 4 7 5 * ATL.Xp 4 0 3 1 * ATL.Xp 2 6 1 7 * ATL.Xp 6 2 5 3
+-/
