Main.lean
@@ -6,5 +6,10 @@ def main : List String → IO Unit
   IO.println s!"loading {fname}"
   let knots ← parseFile fname
   IO.println s!"loaded {knots.size} knots"
+  for (name, pd) in knots do
+    IO.println s!"---\ncalculating for {name}"
+    IO.println s!"{pd}"
+    let p := arrow_poly pd
+    IO.println s!"{p}"
 | _ =>
   throw <| IO.userError "Expecting exactly one argument"
